Update W9.v

plf/W9.v
@@ -1,7 +1,7 @@
 (**
 
 Hoare Logic
-Ref.: Software Foundations, Volume 2, Hoare2.v
+Ref.: Software Foundations, Volume 2, Hoare2.v, SmallStep.v
 
 *)
 
@@ -466,3 +466,385 @@ Example subtract_slowly_dec (m : nat) (n : nat) : decorated :=
 Example vc_subtract_slowly_dec : forall m n, 
 verification_conditions_from (subtract_slowly_dec m n).
 Proof. verify_assertion. Qed. 
+
+
+(**
+Small-step operational semantics
+--------------------------------------
+
+- The evaluation rules that we have seen so far for the IMP
+language are known as 'big-step' operational semantics.
+- [st =[c]=> st'] directly relates the final state st' to the 
+initial state st.
+- Good for whole program reasoning.
+- However, we would like to expose the intermediate states that
+would be required to reach the final state.
+- Useful for finding errors and expressing semantics of concurrent
+programs
+- This is formalized using 'small-step' semantics.
+
+We will demonstrate small-step semantics with a toy language first,
+and then move to IMP.
+*)
+
+Inductive tm : Type :=
+  | C : nat -> tm         (* Constant *)
+  | P : tm -> tm -> tm.   (* Plus *)
+
+Fixpoint evalF (t : tm) : nat :=
+  match t with
+  | C n => n
+  | P t1 t2 => evalF t1 + evalF t2
+  end.
+
+Reserved Notation " t '==>' n " (at level 50, left associativity).
+
+Inductive eval : tm -> nat -> Prop :=
+  | E_C : forall n,
+      C n ==> n
+  | E_P : forall t1 t2 n1 n2,
+      t1 ==> n1 ->
+      t2 ==> n2 ->
+      P t1 t2 ==> (n1 + n2)
+
+where " t '==>' n " := (eval t n).
+
+Module SimpleArith1.
+
+Reserved Notation " t '-->' t' " (at level 40).
+
+Inductive step : tm -> tm -> Prop :=
+  | ST_PCC : forall n1 n2,
+      P (C n1) (C n2) --> C (n1 + n2)
+  | ST_P1 : forall t1 t1' t2,
+      t1 --> t1' ->
+      P t1 t2 --> P t1' t2
+  | ST_P2 : forall n1 t2 t2',
+      t2 --> t2' ->
+      P (C n1) t2 --> P (C n1) t2'
+
+  where " t '-->' t' " := (step t t').
+
+(**
+- Notice that step is a binary relation over terms, as compared to the
+eval relation which related a term with a number.
+- Can be thought of a as a single step in an abstract machine which
+is trying to evaluate a term.
+*)
+
+Example test_step_1 :
+      P
+        (P (C 1) (C 3))
+        (P (C 2) (C 4))
+      -->
+      P
+        (C 4)
+        (P (C 2) (C 4)).
+Proof.
+  apply ST_P1. apply ST_PCC.  Qed.
+
+Example test_step_2 :
+      P
+        (C 0)
+        (P
+          (C 2)
+          (P (C 1) (C 3)))
+      -->
+      P
+        (C 0)
+        (P
+          (C 2)
+          (C 4)).
+Proof. apply ST_P2. apply ST_P2. apply ST_PCC. Qed. 
+
+End SimpleArith1.
+
+(**
+We now define the concept of a value, which a special kind of term
+which cannot take a step.
+*)
+
+Inductive value : tm -> Prop :=
+  | v_C : forall n, value (C n).
+
+  Reserved Notation " t '-->' t' " (at level 40).
+
+Inductive step : tm -> tm -> Prop :=
+  | ST_PCC : forall n1 n2,
+          P (C n1) (C n2)
+      --> C (n1 + n2)
+  | ST_P1 : forall t1 t1' t2,
+        t1 --> t1' ->
+        P t1 t2 --> P t1' t2
+  | ST_P2 : forall v1 t2 t2',
+        value v1 ->                     (* <--- new *)
+        t2 --> t2' ->
+        P v1 t2 --> P v1 t2'
+
+  where " t '-->' t' " := (step t t').
+
+Theorem step_deterministic: forall (x y1 y2 : tm),
+  step x y1 -> step x y2 -> y1 = y2.
+Proof. intros x y1 y2 Hy1. generalize dependent y2. induction Hy1; intros y2 Hy2.
+  - inversion Hy2; subst.
+    -- reflexivity.
+    -- inversion H2.
+    -- inversion H3.
+  - inversion Hy2; subst.
+    -- inversion Hy1.
+    -- apply IHHy1 in H2. rewrite H2. reflexivity.
+    -- destruct H1. inversion Hy1.
+  - inversion Hy2; subst.
+    -- inversion Hy1.
+    -- destruct H. inversion H3.
+    -- apply IHHy1 in H4. rewrite H4. reflexivity.
+Qed.
+
+(** While the single-step relation that we have defined is deterministic,
+it is possible to define non-deterministic small step operational
+semantics *)
+
+Module NonDetStep.
+
+Inductive step : tm -> tm -> Prop :=
+  | ST_PCC : forall n1 n2,
+          P (C n1) (C n2)
+      --> C (n1 + n2)
+  | ST_P1 : forall t1 t1' t2,
+        t1 --> t1' ->
+        P t1 t2 --> P t1' t2
+  | ST_P2 : forall t1 t2 t2',                    
+        t2 --> t2' ->
+        P t1 t2 --> P t1 t2'
+
+  where " t '-->' t' " := (step t t').
+
+Theorem step_non_deteministic: exists (x y1 y2 : tm),
+  x --> y1 /\ x --> y2 /\ y1 <> y2.
+Proof. exists (P (P (C 1) (C 1)) (P (C 1) (C 1))).
+  exists (P (C 2) (P (C 1) (C 1))). exists (P (P (C 1) (C 1)) (C 2)).
+  split.
+  - apply ST_P1. constructor.
+  - split. 
+    -- apply ST_P2. constructor.
+    -- unfold not; intros; discriminate H.
+Qed.
+
+End NonDetStep.
+
+
+
+(**
+We can also prove a 'strong progress' property: Either a term is a
+value, or it can take a step.
+*)
+
+Theorem strong_progress : forall x,
+  value x \/ (exists x', x --> x').
+Proof.
+  induction x.
+  - left. constructor.
+  - destruct IHx1 as [Iv1 | [x' It1]].
+    -- destruct IHx2 as [Iv2 | [x' It2]].
+       * inversion Iv1; subst. inversion Iv2; subst. 
+         right. exists (C (n + n0)). constructor.
+       * right. exists (P x1 x'). constructor; assumption.
+    -- right. exists (P x' x2). constructor; assumption.
+Qed.   
+
+(**
+A term which cannot progress is are said to be in normal form.
+We formalize this below:
+*)
+
+Definition relation (X : Type) := X -> X -> Prop.
+
+Definition normal_form {X : Type}
+              (R : relation X) (t : X) : Prop :=
+  ~ exists t', R t t'.
+
+(** For our toy language, values are exactly those terms which are in
+normal form. However, this may not be true in general.
+ *)
+
+Lemma value_is_nf : forall v,
+  value v -> normal_form step v.
+Proof.
+  unfold normal_form. intros v H contra.
+  destruct contra. destruct H. inversion H0.
+Qed.
+
+Lemma nf_is_value : forall t,
+  normal_form step t -> value t.
+Proof. (* a corollary of [strong_progress]... *)
+  unfold normal_form. intros t H.
+  assert (G : value t \/ exists t', t --> t').
+  { apply strong_progress. }
+  destruct G as [G | G].
+  - (* l *) apply G.
+  - (* r *) contradiction.
+Qed.
+
+(** Multi-step reduction 
+
+We would like to relate terms t -->* t' where t' can be obtained by
+performing multiple (zero or more) steps of reduction from t.
+
+*)
+
+Inductive multi {X : Type} (R : relation X) : relation X :=
+| multi_refl : forall (x : X), multi R x x
+| multi_step : forall (x y z : X),
+                  R x y ->
+                  multi R y z ->
+                  multi R x z.
+
+Notation " t '-->*' t' " := (multi step t t') (at level 40).
+
+Definition normal_form_of {X : Type} (R : relation X)  (t t' : X) :=
+  ((multi R) t t' /\ normal_form R t').
+
+(**
+Since the step relation is deterministic, every term also has a
+unique normal form:
+*)
+
+Theorem normal_forms_unique: forall (x y1 y2 : tm),
+ normal_form_of step x y1 -> normal_form_of step x y2 -> y1 = y2.
+Proof. unfold normal_form_of. intros. destruct H as [H11 H12].
+  destruct H0 as [H21 H22].
+  induction H11.
+  - apply nf_is_value in H12. inversion H21; subst. reflexivity.
+    destruct H12. inversion H.
+  - apply IHmulti. assumption. inversion H21; subst.
+    -- apply nf_is_value in H22. destruct H22. inversion H.
+    -- replace y with y0. assumption. apply step_deterministic with (x := x); assumption.
+Qed.     
+
+(** We can also say something stronger: for our language, for any 
+term, its normal form can be obtained by applying a *finite* number
+of reduction steps. Such a language is called normalizing*)
+      
+Definition normalizing {X : Type} (R : relation X) :=
+  forall t, exists t', normal_form_of R t t'.
+
+(** Homework: Prove normalizing step *)
+
+(** Homework: We can also prove that the big step and small step reductions are equivalent to each other:
+
+t ==> n -> t -->* C n.
+*)
+
+(**
+Small step semantics for IMP
+
+*)
+
+Inductive aval : aexp -> Prop :=
+  | av_num : forall n, aval (ANum n).
+
+
+Reserved Notation " a '/' st '-->a' a' "
+                  (at level 40, st at next level, left associativity).
+Inductive astep (st : state) : aexp -> aexp -> Prop :=
+  | AS_Id : forall (i : string),
+      i / st -->a ANum (st i)
+  | AS_P1 : forall a1 a1' a2,
+      a1 / st -->a a1' ->
+      <{ a1 + a2 }> / st -->a <{ a1' + a2 }>
+  | AS_P2 : forall v1 a2 a2',
+      aval v1 ->
+      a2 / st -->a a2' ->
+      <{ v1 + a2 }>  / st -->a <{ v1 + a2' }>
+  | AS_P : forall (v1 v2 : nat),
+      <{ v1 + v2 }> / st -->a ANum (v1 + v2)
+  | AS_Minus1 : forall a1 a1' a2,
+      a1 / st -->a a1' ->
+      <{ a1 - a2 }> / st -->a <{ a1' - a2 }>
+  | AS_Minus2 : forall v1 a2 a2',
+      aval v1 ->
+      a2 / st -->a a2' ->
+      <{ v1 - a2 }>  / st -->a <{ v1 - a2' }>
+  | AS_Minus : forall (v1 v2 : nat),
+      <{ v1 - v2 }> / st -->a ANum (v1 - v2)
+  | AS_Mult1 : forall a1 a1' a2,
+      a1 / st -->a a1' ->
+      <{ a1 * a2 }> / st -->a <{ a1' * a2 }>
+  | AS_Mult2 : forall v1 a2 a2',
+      aval v1 ->
+      a2 / st -->a a2' ->
+      <{ v1 * a2 }>  / st -->a <{ v1 * a2' }>
+  | AS_Mult : forall (v1 v2 : nat),
+      <{ v1 * v2 }> / st -->a ANum (v1 * v2)
+
+    where " a '/' st '-->a' a' " := (astep st a a').
+
+Reserved Notation " b '/' st '-->b' b' "
+                  (at level 40, st at next level, left associativity).
+Inductive bstep (st : state) : bexp -> bexp -> Prop :=
+| BS_Eq1 : forall a1 a1' a2,
+    a1 / st -->a a1' ->
+    <{ a1 = a2 }> / st -->b <{ a1' = a2 }>
+| BS_Eq2 : forall v1 a2 a2',
+    aval v1 ->
+    a2 / st -->a a2' ->
+    <{ v1 = a2 }> / st -->b <{ v1 = a2' }>
+| BS_Eq : forall (v1 v2 : nat),
+    <{ v1 = v2 }> / st -->b
+    (if (v1 =? v2) then BTrue else BFalse)
+| BS_LtEq1 : forall a1 a1' a2,
+    a1 / st -->a a1' ->
+    <{ a1 <= a2 }> / st -->b <{ a1' <= a2 }>
+| BS_LtEq2 : forall v1 a2 a2',
+    aval v1 ->
+    a2 / st -->a a2' ->
+    <{ v1 <= a2 }> / st -->b <{ v1 <= a2' }>
+| BS_LtEq : forall (v1 v2 : nat),
+    <{ v1 <= v2 }> / st -->b
+    (if (v1 <=? v2) then BTrue else BFalse)
+| BS_NotStep : forall b1 b1',
+    b1 / st -->b b1' ->
+    <{ ~ b1 }> / st -->b <{ ~ b1' }>
+| BS_NotTrue  : <{ ~ true }> / st  -->b <{ false }>
+| BS_NotFalse : <{ ~ false }> / st -->b <{ true }>
+| BS_AndStep : forall b1 b1' b2,
+    b1 / st -->b b1' ->
+    <{ b1 && b2 }> / st -->b <{ b1' && b2 }>
+| BS_AndTrueStep : forall b2 b2',
+    b2 / st -->b b2' ->
+    <{ true && b2 }> / st -->b <{ true && b2' }>
+| BS_AndFalse : forall b2,
+    <{ false && b2 }> / st -->b <{ false }>
+| BS_AndTrueTrue  : <{ true && true  }> / st -->b <{ true }>
+| BS_AndTrueFalse : <{ true && false }> / st -->b <{ false }>
+
+where " b '/' st '-->b' b' " := (bstep st b b').
+
+Reserved Notation " t '/' st '-->' t' '/' st' "
+                  (at level 40, st at next level, t' at next level, left associativity).
+Inductive cstep : (com * state) -> (com * state) -> Prop :=
+  | CS_AsgnStep : forall st i a1 a1',
+      a1 / st -->a a1' ->
+      <{ i := a1 }> / st --> <{ i := a1' }> / st
+  | CS_Asgn : forall st i (n : nat),
+      <{ i := n }> / st --> <{ skip }> / (i !-> n ; st)
+  | CS_SeqStep : forall st c1 c1' st' c2,
+      c1 / st --> c1' / st' ->
+      <{ c1 ; c2 }> / st --> <{ c1' ; c2 }> / st'
+  | CS_SeqFinish : forall st c2,
+      <{ skip ; c2 }> / st --> c2 / st
+  | CS_IfStep : forall st b1 b1' c1 c2,
+      b1 / st -->b b1' ->
+      <{ if b1 then c1 else c2 end }> / st
+      -->
+      <{ if b1' then c1 else c2 end }> / st
+  | CS_IfTrue : forall st c1 c2,
+      <{ if true then c1 else c2 end }> / st --> c1 / st
+  | CS_IfFalse : forall st c1 c2,
+      <{ if false then c1 else c2 end }> / st --> c2 / st
+  | CS_While : forall st b1 c1,
+      <{ while b1 do c1 end }> / st
+      -->
+      <{ if b1 then c1; while b1 do c1 end else skip end }> / st
+
+  where " t '/' st '-->' t' '/' st' " := (cstep (t,st) (t',st')).
